libcrux-ml-kem/proofs/fstar/extraction/Libcrux_ml_kem.Vector.Avx2.Arithmetic.fst
@@ -85,21 +85,34 @@ let sub (lhs rhs: Libcrux_intrinsics.Avx2_extract.t_Vec256) =
   in
   result
 
+#push-options "--z3rlimit 100"
+
 let barrett_reduce (vector: Libcrux_intrinsics.Avx2_extract.t_Vec256) =
-  let t:Libcrux_intrinsics.Avx2_extract.t_Vec256 =
+  let t0:Libcrux_intrinsics.Avx2_extract.t_Vec256 =
     Libcrux_intrinsics.Avx2_extract.mm256_mulhi_epi16 vector
       (Libcrux_intrinsics.Avx2_extract.mm256_set1_epi16 v_BARRETT_MULTIPLIER
         <:
         Libcrux_intrinsics.Avx2_extract.t_Vec256)
   in
-  let t:Libcrux_intrinsics.Avx2_extract.t_Vec256 =
-    Libcrux_intrinsics.Avx2_extract.mm256_add_epi16 t
+  let _:Prims.unit =
+    assert (forall i.
+          get_lane t0 i ==
+          (cast (((cast (get_lane vector i) <: i32) *. (cast v_BARRETT_MULTIPLIER <: i32)) >>! 16l)
+            <:
+            i16))
+  in
+  let t1:Libcrux_intrinsics.Avx2_extract.t_Vec256 =
+    Libcrux_intrinsics.Avx2_extract.mm256_add_epi16 t0
       (Libcrux_intrinsics.Avx2_extract.mm256_set1_epi16 512s
         <:
         Libcrux_intrinsics.Avx2_extract.t_Vec256)
   in
+  let _:Prims.unit = assert (forall i. get_lane t1 i == get_lane t0 i +. 512s) in
   let quotient:Libcrux_intrinsics.Avx2_extract.t_Vec256 =
-    Libcrux_intrinsics.Avx2_extract.mm256_srai_epi16 10l t
+    Libcrux_intrinsics.Avx2_extract.mm256_srai_epi16 10l t1
+  in
+  let _:Prims.unit =
+    assert (forall i. get_lane quotient i == (((get_lane t1 i) <: i16) >>! (10l <: i32)))
   in
   let quotient_times_field_modulus:Libcrux_intrinsics.Avx2_extract.t_Vec256 =
     Libcrux_intrinsics.Avx2_extract.mm256_mullo_epi16 quotient
@@ -107,38 +120,153 @@ let barrett_reduce (vector: Libcrux_intrinsics.Avx2_extract.t_Vec256) =
         <:
         Libcrux_intrinsics.Avx2_extract.t_Vec256)
   in
-  Libcrux_intrinsics.Avx2_extract.mm256_sub_epi16 vector quotient_times_field_modulus
+  let _:Prims.unit =
+    assert (forall i.
+          get_lane quotient_times_field_modulus i ==
+          get_lane quotient i *. Libcrux_ml_kem.Vector.Traits.v_FIELD_MODULUS)
+  in
+  let result:Libcrux_intrinsics.Avx2_extract.t_Vec256 =
+    Libcrux_intrinsics.Avx2_extract.mm256_sub_epi16 vector quotient_times_field_modulus
+  in
+  let _:Prims.unit =
+    assert (forall i.
+          get_lane result i == get_lane vector i -. get_lane quotient_times_field_modulus i);
+    assert (forall i. get_lane result i == Spec.Utils.barrett_red (get_lane vector i));
+    assert (forall i. v (get_lane result i) % 3329 == v (get_lane vector i) % 3329);
+    assert (forall i. Spec.Utils.is_i16b 3328 (get_lane result i));
+    assert (forall (i: nat). i < 16 ==> Spec.Utils.is_i16b 3328 (get_lane result i));
+    assert (Spec.Utils.is_i16b_array 3328 (Libcrux_intrinsics.Avx2_extract.vec256_as_i16x16 result))
+  in
+  result
+
+#pop-options
+
+#push-options "--z3rlimit 100"
 
 let cond_subtract_3329_ (vector: Libcrux_intrinsics.Avx2_extract.t_Vec256) =
   let field_modulus:Libcrux_intrinsics.Avx2_extract.t_Vec256 =
     Libcrux_intrinsics.Avx2_extract.mm256_set1_epi16 Libcrux_ml_kem.Vector.Traits.v_FIELD_MODULUS
   in
+  let _:Prims.unit = assert (forall i. get_lane field_modulus i == 3329s) in
   let vv_minus_field_modulus:Libcrux_intrinsics.Avx2_extract.t_Vec256 =
     Libcrux_intrinsics.Avx2_extract.mm256_sub_epi16 vector field_modulus
+  in
+  let _:Prims.unit =
+    assert (forall i. get_lane vv_minus_field_modulus i == get_lane vector i -. 3329s)
   in
   let sign_mask:Libcrux_intrinsics.Avx2_extract.t_Vec256 =
     Libcrux_intrinsics.Avx2_extract.mm256_srai_epi16 15l vv_minus_field_modulus
   in
+  let _:Prims.unit =
+    assert (forall i. get_lane sign_mask i == (get_lane vv_minus_field_modulus i >>! 15l))
+  in
   let conditional_add_field_modulus:Libcrux_intrinsics.Avx2_extract.t_Vec256 =
     Libcrux_intrinsics.Avx2_extract.mm256_and_si256 sign_mask field_modulus
+  in
+  let _:Prims.unit =
+    assert (forall i. get_lane conditional_add_field_modulus i == (get_lane sign_mask i &. 3329s))
   in
   let result:Libcrux_intrinsics.Avx2_extract.t_Vec256 =
     Libcrux_intrinsics.Avx2_extract.mm256_add_epi16 vv_minus_field_modulus
       conditional_add_field_modulus
   in
-  let result:Libcrux_intrinsics.Avx2_extract.t_Vec256 = result in
-  let _:Prims.unit = admit () (* Panic freedom *) in
+  let _:Prims.unit =
+    assert (forall i.
+          get_lane result i ==
+          (get_lane vv_minus_field_modulus i +. get_lane conditional_add_field_modulus i));
+    assert (forall i. get_lane result i == Spec.Utils.cond_sub (get_lane vector i));
+    assert (forall i.
+          get_lane result i ==
+          (if (get_lane vector i) >=. 3329s then get_lane vector i -! 3329s else get_lane vector i))
+  in
   result
+
+#pop-options
+
+#push-options "--z3rlimit 100"
 
 let montgomery_multiply_by_constant
       (vector: Libcrux_intrinsics.Avx2_extract.t_Vec256)
       (constant: i16)
      =
-  let constant:Libcrux_intrinsics.Avx2_extract.t_Vec256 =
+  let vec_constant:Libcrux_intrinsics.Avx2_extract.t_Vec256 =
     Libcrux_intrinsics.Avx2_extract.mm256_set1_epi16 constant
   in
+  let _:Prims.unit = assert (forall i. get_lane vec_constant i == constant) in
   let value_low:Libcrux_intrinsics.Avx2_extract.t_Vec256 =
-    Libcrux_intrinsics.Avx2_extract.mm256_mullo_epi16 vector constant
+    Libcrux_intrinsics.Avx2_extract.mm256_mullo_epi16 vector vec_constant
+  in
+  let _:Prims.unit = assert (forall i. get_lane value_low i == get_lane vector i *. constant) in
+  let k:Libcrux_intrinsics.Avx2_extract.t_Vec256 =
+    Libcrux_intrinsics.Avx2_extract.mm256_mullo_epi16 value_low
+      (Libcrux_intrinsics.Avx2_extract.mm256_set1_epi16 (cast (Libcrux_ml_kem.Vector.Traits.v_INVERSE_OF_MODULUS_MOD_MONTGOMERY_R
+                <:
+                u32)
+            <:
+            i16)
+        <:
+        Libcrux_intrinsics.Avx2_extract.t_Vec256)
+  in
+  let _:Prims.unit = assert (forall i. get_lane k i == get_lane value_low i *. (neg 3327s)) in
+  let modulus:Libcrux_intrinsics.Avx2_extract.t_Vec256 =
+    Libcrux_intrinsics.Avx2_extract.mm256_set1_epi16 Libcrux_ml_kem.Vector.Traits.v_FIELD_MODULUS
+  in
+  let _:Prims.unit = assert (forall i. get_lane modulus i == 3329s) in
+  let k_times_modulus:Libcrux_intrinsics.Avx2_extract.t_Vec256 =
+    Libcrux_intrinsics.Avx2_extract.mm256_mulhi_epi16 k modulus
+  in
+  let _:Prims.unit =
+    assert (Libcrux_intrinsics.Avx2_extract.vec256_as_i16x16 k_times_modulus ==
+        Spec.Utils.map2 (fun x y -> cast (((cast x <: i32) *. (cast y <: i32)) >>! 16l) <: i16)
+          (Libcrux_intrinsics.Avx2_extract.vec256_as_i16x16 k)
+          (Libcrux_intrinsics.Avx2_extract.vec256_as_i16x16 modulus));
+    assert (forall i.
+          get_lane k_times_modulus i ==
+          (cast (((cast (get_lane k i) <: i32) *. (cast (get_lane modulus i) <: i32)) >>! 16l)
+            <:
+            i16))
+  in
+  let value_high:Libcrux_intrinsics.Avx2_extract.t_Vec256 =
+    Libcrux_intrinsics.Avx2_extract.mm256_mulhi_epi16 vector vec_constant
+  in
+  let _:Prims.unit =
+    assert (forall i.
+          get_lane value_high i ==
+          (cast (((cast (get_lane vector i) <: i32) *. (cast (get_lane vec_constant i) <: i32)) >>!
+                16l)
+            <:
+            i16))
+  in
+  let result:Libcrux_intrinsics.Avx2_extract.t_Vec256 =
+    Libcrux_intrinsics.Avx2_extract.mm256_sub_epi16 value_high k_times_modulus
+  in
+  let _:Prims.unit =
+    Spec.Utils.lemma_range_at_percent 3329 (pow2 32);
+    assert (v (cast 3329s <: i32) == (3329 @% pow2 32));
+    assert (v (cast 3329s <: i32) == 3329);
+    assert ((cast 3329s <: i32) == 3329l);
+    assert (forall i. get_lane result i == (get_lane value_high i) -. (get_lane k_times_modulus i));
+    assert (forall i. get_lane result i == Spec.Utils.mont_mul_red_i16 (get_lane vector i) constant);
+    assert (forall i. Spec.Utils.is_i16b 3329 (get_lane result i));
+    assert (forall i. Spec.Utils.is_i16b (3328 + 1665) (get_lane result i));
+    assert (forall (i: nat). i < 16 ==> Spec.Utils.is_i16b (3328 + 1665) (get_lane result i));
+    assert (Spec.Utils.is_i16b_array (3328 + 1665)
+          (Libcrux_intrinsics.Avx2_extract.vec256_as_i16x16 result));
+    assert (forall i.
+          v (get_lane result i) % 3329 == ((v (get_lane vector i) * v constant * 169) % 3329))
+  in
+  result
+
+#pop-options
+
+#push-options "--z3rlimit 100"
+
+let montgomery_multiply_by_constants (vec constants: Libcrux_intrinsics.Avx2_extract.t_Vec256) =
+  let value_low:Libcrux_intrinsics.Avx2_extract.t_Vec256 =
+    Libcrux_intrinsics.Avx2_extract.mm256_mullo_epi16 vec constants
+  in
+  let _:Prims.unit =
+    assert (forall i. get_lane value_low i == get_lane vec i *. get_lane constants i)
   in
   let k:Libcrux_intrinsics.Avx2_extract.t_Vec256 =
     Libcrux_intrinsics.Avx2_extract.mm256_mullo_epi16 value_low
@@ -150,45 +278,67 @@ let montgomery_multiply_by_constant
         <:
         Libcrux_intrinsics.Avx2_extract.t_Vec256)
   in
+  let _:Prims.unit = assert (forall i. get_lane k i == get_lane value_low i *. (neg 3327s)) in
+  let modulus:Libcrux_intrinsics.Avx2_extract.t_Vec256 =
+    Libcrux_intrinsics.Avx2_extract.mm256_set1_epi16 Libcrux_ml_kem.Vector.Traits.v_FIELD_MODULUS
+  in
+  let _:Prims.unit = assert (forall i. get_lane modulus i == 3329s) in
   let k_times_modulus:Libcrux_intrinsics.Avx2_extract.t_Vec256 =
-    Libcrux_intrinsics.Avx2_extract.mm256_mulhi_epi16 k
-      (Libcrux_intrinsics.Avx2_extract.mm256_set1_epi16 Libcrux_ml_kem.Vector.Traits.v_FIELD_MODULUS
-        <:
-        Libcrux_intrinsics.Avx2_extract.t_Vec256)
+    Libcrux_intrinsics.Avx2_extract.mm256_mulhi_epi16 k modulus
   in
-  let value_high:Libcrux_intrinsics.Avx2_extract.t_Vec256 =
-    Libcrux_intrinsics.Avx2_extract.mm256_mulhi_epi16 vector constant
-  in
-  Libcrux_intrinsics.Avx2_extract.mm256_sub_epi16 value_high k_times_modulus
-
-let montgomery_multiply_by_constants (v c: Libcrux_intrinsics.Avx2_extract.t_Vec256) =
-  let value_low:Libcrux_intrinsics.Avx2_extract.t_Vec256 =
-    Libcrux_intrinsics.Avx2_extract.mm256_mullo_epi16 v c
-  in
-  let k:Libcrux_intrinsics.Avx2_extract.t_Vec256 =
-    Libcrux_intrinsics.Avx2_extract.mm256_mullo_epi16 value_low
-      (Libcrux_intrinsics.Avx2_extract.mm256_set1_epi16 (cast (Libcrux_ml_kem.Vector.Traits.v_INVERSE_OF_MODULUS_MOD_MONTGOMERY_R
-                <:
-                u32)
+  let _:Prims.unit =
+    assert (Libcrux_intrinsics.Avx2_extract.vec256_as_i16x16 k_times_modulus ==
+        Spec.Utils.map2 (fun x y -> cast (((cast x <: i32) *. (cast y <: i32)) >>! 16l) <: i16)
+          (Libcrux_intrinsics.Avx2_extract.vec256_as_i16x16 k)
+          (Libcrux_intrinsics.Avx2_extract.vec256_as_i16x16 modulus));
+    assert (forall i.
+          get_lane k_times_modulus i ==
+          (cast (((cast (get_lane k i) <: i32) *. (cast (get_lane modulus i) <: i32)) >>! 16l)
             <:
-            i16)
-        <:
-        Libcrux_intrinsics.Avx2_extract.t_Vec256)
-  in
-  let k_times_modulus:Libcrux_intrinsics.Avx2_extract.t_Vec256 =
-    Libcrux_intrinsics.Avx2_extract.mm256_mulhi_epi16 k
-      (Libcrux_intrinsics.Avx2_extract.mm256_set1_epi16 Libcrux_ml_kem.Vector.Traits.v_FIELD_MODULUS
-        <:
-        Libcrux_intrinsics.Avx2_extract.t_Vec256)
+            i16))
   in
   let value_high:Libcrux_intrinsics.Avx2_extract.t_Vec256 =
-    Libcrux_intrinsics.Avx2_extract.mm256_mulhi_epi16 v c
+    Libcrux_intrinsics.Avx2_extract.mm256_mulhi_epi16 vec constants
   in
-  Libcrux_intrinsics.Avx2_extract.mm256_sub_epi16 value_high k_times_modulus
+  let _:Prims.unit =
+    assert (forall i.
+          get_lane value_high i ==
+          (cast (((cast (get_lane vec i) <: i32) *. (cast (get_lane constants i) <: i32)) >>! 16l)
+            <:
+            i16))
+  in
+  let result:Libcrux_intrinsics.Avx2_extract.t_Vec256 =
+    Libcrux_intrinsics.Avx2_extract.mm256_sub_epi16 value_high k_times_modulus
+  in
+  let _:Prims.unit =
+    Spec.Utils.lemma_range_at_percent 3329 (pow2 32);
+    assert (v (cast 3329s <: i32) == (3329 @% pow2 32));
+    assert (v (cast 3329s <: i32) == 3329);
+    assert ((cast 3329s <: i32) == 3329l);
+    assert (forall i. get_lane result i == (get_lane value_high i) -. (get_lane k_times_modulus i));
+    assert (forall i.
+          get_lane result i == Spec.Utils.mont_mul_red_i16 (get_lane vec i) (get_lane constants i));
+    assert (forall i. Spec.Utils.is_i16b 3329 (get_lane result i));
+    assert (forall i. Spec.Utils.is_i16b (3328 + 1665) (get_lane result i));
+    assert (forall (i: nat). i < 16 ==> Spec.Utils.is_i16b (3328 + 1665) (get_lane result i));
+    assert (Spec.Utils.is_i16b_array (3328 + 1665)
+          (Libcrux_intrinsics.Avx2_extract.vec256_as_i16x16 result));
+    assert (forall i.
+          v (get_lane result i) % 3329 ==
+          ((v (get_lane vec i) * v (get_lane constants i) * 169) % 3329))
+  in
+  result
 
-let montgomery_multiply_m128i_by_constants (v c: Libcrux_intrinsics.Avx2_extract.t_Vec128) =
+#pop-options
+
+#push-options "--z3rlimit 100"
+
+let montgomery_multiply_m128i_by_constants (vec constants: Libcrux_intrinsics.Avx2_extract.t_Vec128) =
   let value_low:Libcrux_intrinsics.Avx2_extract.t_Vec128 =
-    Libcrux_intrinsics.Avx2_extract.mm_mullo_epi16 v c
+    Libcrux_intrinsics.Avx2_extract.mm_mullo_epi16 vec constants
+  in
+  let _:Prims.unit =
+    assert (forall i. get_lane128 value_low i == get_lane128 vec i *. get_lane128 constants i)
   in
   let k:Libcrux_intrinsics.Avx2_extract.t_Vec128 =
     Libcrux_intrinsics.Avx2_extract.mm_mullo_epi16 value_low
@@ -200,20 +350,65 @@ let montgomery_multiply_m128i_by_constants (v c: Libcrux_intrinsics.Avx2_extract
         <:
         Libcrux_intrinsics.Avx2_extract.t_Vec128)
   in
+  let _:Prims.unit = assert (forall i. get_lane128 k i == get_lane128 value_low i *. (neg 3327s)) in
+  let modulus:Libcrux_intrinsics.Avx2_extract.t_Vec128 =
+    Libcrux_intrinsics.Avx2_extract.mm_set1_epi16 Libcrux_ml_kem.Vector.Traits.v_FIELD_MODULUS
+  in
+  let _:Prims.unit = assert (forall i. get_lane128 modulus i == 3329s) in
   let k_times_modulus:Libcrux_intrinsics.Avx2_extract.t_Vec128 =
-    Libcrux_intrinsics.Avx2_extract.mm_mulhi_epi16 k
-      (Libcrux_intrinsics.Avx2_extract.mm_set1_epi16 Libcrux_ml_kem.Vector.Traits.v_FIELD_MODULUS
-        <:
-        Libcrux_intrinsics.Avx2_extract.t_Vec128)
+    Libcrux_intrinsics.Avx2_extract.mm_mulhi_epi16 k modulus
+  in
+  let _:Prims.unit =
+    assert (Libcrux_intrinsics.Avx2_extract.vec128_as_i16x8 k_times_modulus ==
+        Spec.Utils.map2 (fun x y -> cast (((cast x <: i32) *. (cast y <: i32)) >>! 16l) <: i16)
+          (Libcrux_intrinsics.Avx2_extract.vec128_as_i16x8 k)
+          (Libcrux_intrinsics.Avx2_extract.vec128_as_i16x8 modulus));
+    assert (forall i.
+          get_lane128 k_times_modulus i ==
+          (cast (((cast (get_lane128 k i) <: i32) *. (cast (get_lane128 modulus i) <: i32)) >>! 16l)
+            <:
+            i16))
   in
   let value_high:Libcrux_intrinsics.Avx2_extract.t_Vec128 =
-    Libcrux_intrinsics.Avx2_extract.mm_mulhi_epi16 v c
+    Libcrux_intrinsics.Avx2_extract.mm_mulhi_epi16 vec constants
   in
-  Libcrux_intrinsics.Avx2_extract.mm_sub_epi16 value_high k_times_modulus
+  let _:Prims.unit =
+    assert (forall i.
+          get_lane128 value_high i ==
+          (cast (((cast (get_lane128 vec i) <: i32) *. (cast (get_lane128 constants i) <: i32)) >>!
+                16l)
+            <:
+            i16))
+  in
+  let result:Libcrux_intrinsics.Avx2_extract.t_Vec128 =
+    Libcrux_intrinsics.Avx2_extract.mm_sub_epi16 value_high k_times_modulus
+  in
+  let _:Prims.unit =
+    Spec.Utils.lemma_range_at_percent 3329 (pow2 32);
+    assert (v (cast 3329s <: i32) == (3329 @% pow2 32));
+    assert (v (cast 3329s <: i32) == 3329);
+    assert ((cast 3329s <: i32) == 3329l);
+    assert (forall i.
+          get_lane128 result i == (get_lane128 value_high i) -. (get_lane128 k_times_modulus i));
+    assert (forall i.
+          get_lane128 result i ==
+          Spec.Utils.mont_mul_red_i16 (get_lane128 vec i) (get_lane128 constants i));
+    assert (forall i. Spec.Utils.is_i16b 3329 (get_lane128 result i));
+    assert (forall i. Spec.Utils.is_i16b (3328 + 1665) (get_lane128 result i));
+    assert (forall (i: nat). i < 8 ==> Spec.Utils.is_i16b (3328 + 1665) (get_lane128 result i));
+    assert (Spec.Utils.is_i16b_array (3328 + 1665)
+          (Libcrux_intrinsics.Avx2_extract.vec128_as_i16x8 result));
+    assert (forall i.
+          v (get_lane128 result i) % 3329 ==
+          ((v (get_lane128 vec i) * v (get_lane128 constants i) * 169) % 3329))
+  in
+  result
 
-let montgomery_reduce_i32s (v: Libcrux_intrinsics.Avx2_extract.t_Vec256) =
+#pop-options
+
+let montgomery_reduce_i32s (vec: Libcrux_intrinsics.Avx2_extract.t_Vec256) =
   let k:Libcrux_intrinsics.Avx2_extract.t_Vec256 =
-    Libcrux_intrinsics.Avx2_extract.mm256_mullo_epi16 v
+    Libcrux_intrinsics.Avx2_extract.mm256_mullo_epi16 vec
       (Libcrux_intrinsics.Avx2_extract.mm256_set1_epi32 (cast (Libcrux_ml_kem.Vector.Traits.v_INVERSE_OF_MODULUS_MOD_MONTGOMERY_R
                 <:
                 u32)
@@ -233,7 +428,7 @@ let montgomery_reduce_i32s (v: Libcrux_intrinsics.Avx2_extract.t_Vec256) =
         Libcrux_intrinsics.Avx2_extract.t_Vec256)
   in
   let value_high:Libcrux_intrinsics.Avx2_extract.t_Vec256 =
-    Libcrux_intrinsics.Avx2_extract.mm256_srli_epi32 16l v
+    Libcrux_intrinsics.Avx2_extract.mm256_srli_epi32 16l vec
   in
   let result:Libcrux_intrinsics.Avx2_extract.t_Vec256 =
     Libcrux_intrinsics.Avx2_extract.mm256_sub_epi16 value_high k_times_modulus
@@ -241,4 +436,8 @@ let montgomery_reduce_i32s (v: Libcrux_intrinsics.Avx2_extract.t_Vec256) =
   let result:Libcrux_intrinsics.Avx2_extract.t_Vec256 =
     Libcrux_intrinsics.Avx2_extract.mm256_slli_epi32 16l result
   in
-  Libcrux_intrinsics.Avx2_extract.mm256_srai_epi32 16l result
+  let result:Libcrux_intrinsics.Avx2_extract.t_Vec256 =
+    Libcrux_intrinsics.Avx2_extract.mm256_srai_epi32 16l result
+  in
+  let _:Prims.unit = admit () (* Panic freedom *) in
+  result
