libcrux-ml-kem/proofs/fstar/extraction/Libcrux_ml_kem.Vector.Avx2.Arithmetic.fsti
@@ -60,7 +60,14 @@ val sub (lhs rhs: Libcrux_intrinsics.Avx2_extract.t_Vec256)
 /// See Section 3.2 of the implementation notes document for an explanation
 /// of this code.
 val barrett_reduce (vector: Libcrux_intrinsics.Avx2_extract.t_Vec256)
-    : Prims.Pure Libcrux_intrinsics.Avx2_extract.t_Vec256 Prims.l_True (fun _ -> Prims.l_True)
+    : Prims.Pure Libcrux_intrinsics.Avx2_extract.t_Vec256
+      (requires
+        Spec.Utils.is_i16b_array 28296 (Libcrux_intrinsics.Avx2_extract.vec256_as_i16x16 vector))
+      (ensures
+        fun result ->
+          let result:Libcrux_intrinsics.Avx2_extract.t_Vec256 = result in
+          Spec.Utils.is_i16b_array 3328 (Libcrux_intrinsics.Avx2_extract.vec256_as_i16x16 result) /\
+          (forall i. i < 16 ==> v (get_lane result i) % 3329 == (v (get_lane vector i) % 3329)))
 
 val cond_subtract_3329_ (vector: Libcrux_intrinsics.Avx2_extract.t_Vec256)
     : Prims.Pure Libcrux_intrinsics.Avx2_extract.t_Vec256
@@ -70,20 +77,66 @@ val cond_subtract_3329_ (vector: Libcrux_intrinsics.Avx2_extract.t_Vec256)
       (ensures
         fun result ->
           let result:Libcrux_intrinsics.Avx2_extract.t_Vec256 = result in
-          Libcrux_intrinsics.Avx2_extract.vec256_as_i16x16 result ==
-          Spec.Utils.map_array (fun x -> if x >=. 3329s then x -! 3329s else x)
-            (Libcrux_intrinsics.Avx2_extract.vec256_as_i16x16 vector))
+          forall i.
+            i < 16 ==>
+            get_lane result i ==
+            (if (get_lane vector i) >=. 3329s then get_lane vector i -! 3329s else get_lane vector i
+            ))
 
 val montgomery_multiply_by_constant
       (vector: Libcrux_intrinsics.Avx2_extract.t_Vec256)
       (constant: i16)
-    : Prims.Pure Libcrux_intrinsics.Avx2_extract.t_Vec256 Prims.l_True (fun _ -> Prims.l_True)
+    : Prims.Pure Libcrux_intrinsics.Avx2_extract.t_Vec256
+      (requires Spec.Utils.is_i16b 3328 constant)
+      (ensures
+        fun result ->
+          let result:Libcrux_intrinsics.Avx2_extract.t_Vec256 = result in
+          Spec.Utils.is_i16b_array (3328 + 1665)
+            (Libcrux_intrinsics.Avx2_extract.vec256_as_i16x16 result) /\
+          (forall i.
+              i < 16 ==>
+              v (get_lane result i) % 3329 == ((v (get_lane vector i) * v constant * 169) % 3329)))
 
-val montgomery_multiply_by_constants (v c: Libcrux_intrinsics.Avx2_extract.t_Vec256)
-    : Prims.Pure Libcrux_intrinsics.Avx2_extract.t_Vec256 Prims.l_True (fun _ -> Prims.l_True)
+val montgomery_multiply_by_constants (vec constants: Libcrux_intrinsics.Avx2_extract.t_Vec256)
+    : Prims.Pure Libcrux_intrinsics.Avx2_extract.t_Vec256
+      (requires
+        Spec.Utils.is_i16b_array 3328 (Libcrux_intrinsics.Avx2_extract.vec256_as_i16x16 constants))
+      (ensures
+        fun result ->
+          let result:Libcrux_intrinsics.Avx2_extract.t_Vec256 = result in
+          Spec.Utils.is_i16b_array (3328 + 1665)
+            (Libcrux_intrinsics.Avx2_extract.vec256_as_i16x16 result) /\
+          (forall i.
+              i < 16 ==>
+              v (get_lane result i) % 3329 ==
+              ((v (get_lane vec i) * v (get_lane constants i) * 169) % 3329)))
 
-val montgomery_multiply_m128i_by_constants (v c: Libcrux_intrinsics.Avx2_extract.t_Vec128)
-    : Prims.Pure Libcrux_intrinsics.Avx2_extract.t_Vec128 Prims.l_True (fun _ -> Prims.l_True)
+val montgomery_multiply_m128i_by_constants (vec constants: Libcrux_intrinsics.Avx2_extract.t_Vec128)
+    : Prims.Pure Libcrux_intrinsics.Avx2_extract.t_Vec128
+      (requires
+        Spec.Utils.is_i16b_array 3328 (Libcrux_intrinsics.Avx2_extract.vec128_as_i16x8 constants))
+      (ensures
+        fun result ->
+          let result:Libcrux_intrinsics.Avx2_extract.t_Vec128 = result in
+          Spec.Utils.is_i16b_array (3328 + 1665)
+            (Libcrux_intrinsics.Avx2_extract.vec128_as_i16x8 result) /\
+          (forall i.
+              i < 8 ==>
+              v (get_lane128 result i) % 3329 ==
+              ((v (get_lane128 vec i) * v (get_lane128 constants i) * 169) % 3329)))
 
-val montgomery_reduce_i32s (v: Libcrux_intrinsics.Avx2_extract.t_Vec256)
-    : Prims.Pure Libcrux_intrinsics.Avx2_extract.t_Vec256 Prims.l_True (fun _ -> Prims.l_True)
+val montgomery_reduce_i32s (vec: Libcrux_intrinsics.Avx2_extract.t_Vec256)
+    : Prims.Pure Libcrux_intrinsics.Avx2_extract.t_Vec256
+      (requires
+        Spec.Utils.is_i16b_array (3328 * pow2 16)
+          (Libcrux_intrinsics.Avx2_extract.vec256_as_i16x16 vec))
+      (ensures
+        fun result ->
+          let result:Libcrux_intrinsics.Avx2_extract.t_Vec256 = result in
+          Spec.Utils.is_i16b_array (3328 + 1665)
+            (Libcrux_intrinsics.Avx2_extract.vec256_as_i16x16 result) /\
+          (Spec.Utils.is_i16b_array (3328 * 3328)
+              (Libcrux_intrinsics.Avx2_extract.vec256_as_i16x16 vec) ==>
+            Spec.Utils.is_i16b_array 3328 (Libcrux_intrinsics.Avx2_extract.vec256_as_i16x16 result)) /\
+          (forall i. i < 16 ==> v (get_lane result i) % 3329 == ((v (get_lane vec i) * 169) % 3329))
+      )
